LambdaS5/coq/LjsCorrectness.v
@@ -752,13 +752,15 @@ Lemma eval_get_obj_attr_correct : forall runs c st oa e1 o,
     runs_type_correct runs ->
     eval_get_obj_attr runs c st e1 oa = result_some o ->
     is_some_value o (runs_type_eval runs c st e1) (fun st' v1 =>
-        exists ptr obj, v1 = value_object ptr /\ 
-            st' \(ptr?) = Some obj /\ 
-            o = out_ter st' (res_value (get_object_oattr obj oa))).
+        exists ptr oas props, v1 = value_object ptr /\ 
+            st' \(ptr?) = Some (object_intro oas props) /\ 
+            o = out_ter st' (res_value (get_oattrs_oattr oas oa))).
 Proof.
     introv IH R. unfolds in R.
     ljs_run_push_post_auto; repeat ljs_is_some_value_munch.
-    ljs_run_inv. eauto.
+    ljs_run_inv. substs. 
+    match goal with obj : object |- _ => destruct obj end.
+    jauto.
 Qed.
 
 Local Hint Constructors object_oattr_valid object_oattr_modifiable.
@@ -768,11 +770,11 @@ Lemma eval_set_obj_attr_correct : forall runs c st oa e1 e2 o,
     eval_set_obj_attr runs c st e1 oa e2 = result_some o ->
     is_some_value o (runs_type_eval runs c st e1) (fun st' v1 =>
         is_some_value o (runs_type_eval runs c st' e2) (fun st'' v2 =>
-            exists ptr obj, v1 = value_object ptr /\
-                st'' \(ptr?) = Some obj /\
+            exists ptr oas props, v1 = value_object ptr /\
+                st'' \(ptr?) = Some (object_intro oas props) /\
                 object_oattr_valid oa v2 /\
-                object_oattr_modifiable obj oa /\
-                o = out_ter (st'' \(ptr := set_object_oattr obj oa v2)) (res_value v2))).
+                object_oattr_modifiable oas oa /\
+                o = out_ter (st'' \(ptr := object_intro (set_oattrs_oattr oas oa v2) props)) (res_value v2))).
 Proof.
     introv IH R. unfolds in R.
     ljs_run_push_post_auto; repeat ljs_is_some_value_munch.
@@ -1136,6 +1138,7 @@ Proof.
     inverts Hy1. inverts Hy2.
     inverts Hy5.
     rewrite read_option_binds_eq in Hy3. 
+    destruct obj.
     eapply red_expr_get_attr_1; eauto.
     (* set_attr *)
     lets H: eval_set_attr_correct IH R. 
@@ -1144,13 +1147,14 @@ Proof.
     destruct H as (ptr&obj&s&Hy1&Hy2&Hy3&H).
     rewrite read_option_binds_eq in Hy3.  
     substs.
+    destruct obj.
     destruct_hyp H.
     eapply red_expr_set_attr_1_add_field; eauto with bag.
     eapply red_expr_set_attr_1; eauto with bag.
     (* get_obj_attr *)
     lets H: eval_get_obj_attr_correct IH R.
     ljs_pretty_advance red_expr_get_obj_attr red_expr_get_obj_attr_1_abort.
-    destruct H as (ptr&obj&Hy1&Hy2&Hy3).
+    destruct H as (ptr&oas&props&Hy1&Hy2&Hy3).
     inverts Hy1. inverts Hy3.
     rewrite read_option_binds_eq in Hy2. 
     eapply red_expr_get_obj_attr_1; eauto.
@@ -1158,8 +1162,8 @@ Proof.
     lets H: eval_set_obj_attr_correct IH R.
     eapply red_expr_set_obj_attr.
     ljs_advance_eval_many.
-    destruct H as (ptr&obj&obj'&Hy1&Hy2&Hy3&Hy4).
-    rewrite read_option_binds_eq in Hy1. substs.
+    destruct H as (ptr&oas&props&Hy1&Hy2&Hy3&Hy4&Hy5).
+    rewrite read_option_binds_eq in Hy2. substs.
     eapply red_expr_set_obj_attr_1; eauto.
     (* get_field *)
     lets H: eval_get_field_correct IH R.
